\documentclass[letterpaper]{article}
\usepackage[margin=1in]{geometry}
\usepackage{amsmath, amssymb}
\usepackage{enumerate}
\usepackage{fancyhdr}

\pagestyle{fancy}
\fancyhead[L]{STAT 542 HW9}
\fancyhead[R]{Xin Yin}

\newcommand{\intii}{\int_{-\infty}^\infty}
\newcommand{\intzi}{\int_0^\infty}
\renewcommand{\arraystretch}{1.5}

\begin{document}
    \section*{4.16}
    \begin{enumerate}
    \item[(c)]
    Let $Z=X+Y, \quad z = 2, 3, \dots$, so $Y=Z-X$.
    \[
    P(X=x, X+Y=z) = P(X=x, Y=z-x) = p(1-p)^{x-1} p(1-p)^{z-x-1} = p^2(1-p)^{z-2}, \quad z = 2, 3, \dots
    \]
    \end{enumerate}
    \section*{4.23}
    \begin{enumerate}[(a)]
    \item
    For the joint pdf of $(X, Y)$,
    \begin{align*}
    f_{X,Y}(x,y) & = \frac{\Gamma(\alpha+\beta)}{\Gamma(\alpha)\Gamma(\beta)} x^{\alpha-1} (1-x)^{\beta-1} \frac{\Gamma(\alpha+\beta+\gamma)}{\Gamma(\alpha+\beta)\Gamma(\gamma)} y^{\alpha+\beta-1} (1-y)^{\gamma-1}
    & 0 < x < 1, \quad 0 < y < 1.
    \end{align*}
    If $U=XY, 0 < u < 1, \quad V=Y, 0 < v < 1$, we have, 
    \[
    X=U/V, \quad Y=V.
    \]
    So the Jacobian is,
    \[
    J = \begin{vmatrix}
    \frac{\partial u/v}{\partial u} & \frac{\partial u/v}{\partial v} \\
    \frac{\partial v}{\partial u} & \frac{\partial v}{\partial v} \\
    \end{vmatrix} = 1/v
    \]

    Then, the joint density for $(U, V)$ is,
    \begin{align*}
    f_{U,V}(u, v) & = f_{X,Y}(uv, v)|J| \\
    & = \frac{\Gamma(\alpha+\beta)}{\Gamma(\alpha)\Gamma(\beta)} \left(\frac{u}{v}\right)^{\alpha-1} (1-\frac{u}{v})^{\beta-1} \frac{\Gamma(\alpha+\beta+\gamma)}{\Gamma(\alpha+\beta)\Gamma(\gamma)} v^{\alpha+\beta-1} (1-v)^{\gamma-1} \frac{1}{v} \\
    \\
    f_U(u) & = \int_0^1 f(u,v)dv \\
    & = \frac{\Gamma(\alpha+\beta+\gamma)}{\Gamma(\alpha)\Gamma(\beta)\Gamma(\gamma)} u^{\alpha-1} \int_0^1 (v-u)^{\beta-1}(1-v)^{\gamma-1} dv \\
    & \text{Let $y = \frac{v-u}{1-u}, \quad dv = d\big((1-u)y+u\big)$},\\
    & = \frac{\Gamma(\alpha+\beta+\gamma)}{\Gamma(\alpha)\Gamma(\beta+\gamma)} u^{\alpha-1} (1-u)^{\beta+\gamma-1} \int_0^1 \frac{\Gamma(\beta+\gamma)}{\Gamma(\beta)\Gamma(\beta)} y^{\beta-1} (1-y)^{\gamma-1} dy \\
    & = \frac{\Gamma(\alpha+\beta+\gamma)}{\Gamma(\alpha)\Gamma(\beta+\gamma)} u^{\alpha-1} (1-u)^{\beta+\gamma-1} 
    \end{align*}
    So, $U \sim \text{Gamma}(\alpha, \beta+\gamma)$.
    \item Similarly, given 
    \[
    \begin{cases}
    U = XY,  \quad 0 < u < 1, \\
    V = X/Y, \quad u < v < \frac{1}{u} < \infty
    \end{cases}
    \]
    , we have, 
    \[
    X = \sqrt{uv}, \quad Y = \sqrt{\frac{u}{v}}.
    \]
    The Jacobian is,
    \[
    J = \begin{vmatrix}
    \frac{\partial \sqrt{uv}}{\partial u} & \frac{\partial \sqrt{uv}}{\partial v} \\
    \frac{\partial \sqrt{u/v}}{\partial \sqrt{u/v}} & \frac{\partial v}{\partial v} \\
    \end{vmatrix} = -\frac{1}{2v}
    \]

    \begin{align*}
    f_{U,V}(u,v) & = f_{X,Y}(\sqrt{uv}, \sqrt{u/v})|J| \\
    & = \frac{\Gamma(\alpha+\beta)}{\Gamma(\alpha)\Gamma(\beta)} (\sqrt{uv})^{\alpha-1}(1-\sqrt{uv})^{\beta-1} \frac{\Gamma(\alpha+\beta+\gamma)}{\Gamma(\alpha+\beta)\Gamma(\gamma)}\left(\sqrt{\frac{u}{v}}\right)^{\alpha+\beta-1}\left(1-\sqrt{\frac{u}{v}}\right)^{\gamma-1} \frac{1}{2v} \\
    & = \frac{\Gamma(\alpha+\beta+\gamma)}{\Gamma(\alpha)\Gamma(\beta)\Gamma(\gamma)} u^{\alpha-1} \left(\sqrt{\frac{u}{v}} -u\right)^{\beta-1} \left(1-\sqrt{\frac{u}{v}}\right)^{\gamma-1} \sqrt{\frac{u}{v}} \frac{1}{2v}\\
    \\
    & \text{Let $y = \frac{\sqrt{u/v}-u}{1-u}, 0 < y < 1, \quad v = \frac{u}{(y(1-u)+u)^2}$},\\
    & dv = \frac{-2u(1-u)}{(y(1-u)+u)^3} dy \\
    f_U(u) & = \frac{\Gamma(\alpha+\beta+\gamma)}{\Gamma(\alpha)\Gamma(\beta+\gamma)} u^{\alpha-1} (1-u)^{\beta+\gamma-2} \int_1^0 \frac{\Gamma(\beta+\gamma)}{\Gamma(\beta)\Gamma(\beta)} y^{\beta-1} (1-y)^{\gamma-1} \frac{(y(1-u)+u)^3}{2u} \frac{-2u(1-u)}{(y(1-u)+u)^3} dy \\
    & = \frac{\Gamma(\alpha+\beta+\gamma)}{\Gamma(\alpha)\Gamma(\beta+\gamma)} u^{\alpha-1} (1-u)^{\beta+\gamma-1} \int_0^1 \frac{\Gamma(\beta+\gamma)}{\Gamma(\beta)\Gamma(\beta)} y^{\beta-1} (1-y)^{\gamma-1} dy \\
    & = \frac{\Gamma(\alpha+\beta+\gamma)}{\Gamma(\alpha)\Gamma(\beta+\gamma)} u^{\alpha-1} (1-u)^{\beta+\gamma-1}\\
    \end{align*}
    So, $f_U(u)$ is the pdf of Gamma$(\alpha, \beta+\gamma)$, again.
    \end{enumerate}

    \section*{4.26}
    \begin{enumerate}[(a)]
    \item
    Since $X$ and $Y$ are independent random variables, we have,
    \[
    f(x,y) = f(x) f(y) = \frac{1}{\lambda} e^{-x/\lambda} \frac{1}{\mu} e^{-y/\mu}, \quad 0 < x, y < \infty
    \]
    
    If $X<Y, \quad Z=\min\{X,Y\} = X, 0 < z=x < y < \infty, \quad W = 1$. Therefore we will have,
    \begin{align*}
    f(z, w) &= P(Z=X \le z, W=1) = \int_0^z \int_x^\infty f(x,y)dydx \\
    & = \int_0^z \frac{1}{\lambda} e^{-x/\lambda} e^{-x/\mu} dx \\
    & = \frac{\mu}{\lambda + \mu} (1- e^{-\frac{\mu+\lambda}{\mu\lambda}z}). 
    \end{align*}
    Otherwise, if $Y<X$, we have,
    \begin{align*}
    F(z, w) &= P(Z=Y \le z, W=0) = \int_0^z \int_y^\infty f(x,y)dxdy \\
    & = \int_0^z \frac{1}{\mu} e^{-y/\mu} e^{-x/\lambda} dy \\
    & = \frac{\lambda}{\lambda + \mu} (1- e^{-\frac{\mu+\lambda}{\mu\lambda}z}). 
    \end{align*}
    \item
    \begin{align*}
    P(Z \le z) & = \sum_{i\in\{0, 1\}} P(Z \le z, W=i) \\
    & = 1- e^{-\frac{\mu+\lambda}{\mu\lambda}z}\\
    \\
    P(W = 1) & = P(X \le Y) = \intzi \int_0^y \frac{1}{\mu} e^{-y/\mu} \frac{1}{\lambda} e^{-x/\lambda} dx dy \\
    & = \frac{\mu}{\mu+\lambda}\\
    \\
    P(W = 0) & = P(Y \le X) = \intzi \int_0^x \frac{1}{\mu} e^{-y/\mu} \frac{1}{\lambda} e^{-x/\lambda} dy dx \\
    & = \frac{\lambda}{\mu+\lambda}\\
    \end{align*}
    We can identify that $P(Z\le z, W=i) = P(Z \le z)P(W = i), \quad i = 0, 1$. So $Z$ and $W$ are independent.
    \end{enumerate}

    \section*{4.28}
    \begin{enumerate}[(a)]
    \item
    Let $U = X/(X+Y), -\infty < u < \infty, \quad V=X+Y, -\infty < v < \infty$, so $X = UV, \quad Y=V(1-U)$.
    The Jacobian is,
    \[
    J = \begin{vmatrix}
    \frac{\partial uv}{\partial u} & \frac{\partial uv}{\partial v} \\
    \frac{\partial v(1-u)}{\partial u} & \frac{\partial v(1-u)}{\partial v} \\
    \end{vmatrix} = v
    \]

    Also, because $X$ and $Y$ are independent standard normal r.v.'s, 
    \begin{align*}
    f(x,y) & = \frac{1}{2\pi} e^{-\frac{x^2+y^2}{2}} \\
    f(u,v) & = f_{X,Y}(X=uv, Y=v(1-u))|J| \\
    & = \frac{1}{2\pi}e^{-\frac{v^2(2u^2-2u+1)}{2}}|v| \\
    f_{X/(X+Y)} = f_U(u) & = \frac{2}{2\pi} \intzi ve^{-\frac{v^2(2u^2-2u+1)}{2}} dv = \frac{1}{2\pi} \frac{1}{u^2-u+1/2} \\
    & = \frac{1}{\pi/2} \frac{1}{1+\left(\frac{(u-1/2)}{1/2}\right)^2}
    \end{align*}
    So, $X/(X+Y)$ has Cauchy$(1/2, 1/2)$ distribution.
    \item Let $Z = X/|Y|, -\infty < z \infty$. Then the cdf for $Z$ is,
    \begin{align*}
    F_Z(z) & = P(Z = X/|Y| \le z) = P(X \le z|Y|) \\
    & = \intii \int_{-\infty}^{z|y|} f_{X} (x) dx f_Y(y) dy \\
    & = \intii F_X(z|y|) f_Y(y) dy = 2 \intzi F_X(zy) f_Y(y) dy \\
    \\
    f_Z(z) & = \frac{d}{dz} 2 \intzi F_X(z) f_Y(y) dy \\
    & = 2 \intzi f_X(zy) y f_Y(y) dy 
    = \intzi \frac{1}{\pi} e^{-\frac{z^2y^2+y^2}{2}} dy \\
    & = \intzi \frac{1}{\pi} e^{-\frac{y^2(z^2+1)}{2}} dy \\
    & = \frac{1}{\pi}\frac{1}{1+z^2}
    \end{align*}
    So, $X/|Y|$ has a Cauchy$(1,1)$ distribution.
    \item If $X_i \stackrel{iid}{\sim} N(0,1), \quad i=1, 2, \dots, k$, 
    \[
    \frac{X_j}{\sum_{i=1}^k X_i} \sim \text{Cauchy}(1/k, 1/k).
    \]
    \end{enumerate}

    \section*{4.30}
    \begin{enumerate}
    \item[(b)] We have shown that,
    \[
    f(x, y) = \frac{1}{\sqrt{2\pi} x} e^{-\frac{(y-x)^2}{2x^2}}.
    \]
    Now let $U=Y/X, -\infty < u < \infty; \quad V=X, 0 < v < 1$, then $Y = UV, X = V$. The Jacobian is,
    \[
    J = \begin{vmatrix}
    \frac{\partial uv}{\partial u} & \frac{\partial uv}{\partial v} \\
    \frac{\partial v}{\partial u} & \frac{\partial v}{\partial v} \\
    \end{vmatrix} = -v
    \]

    Therefore,
    \begin{align*}
    f(u,v) & = f(X=v, Y=uv)|J| \\
    & = \frac{1}{\sqrt{2\pi}v} v e^{-\frac{(uv-v)^2}{2v^2}} \\
    & = \frac{1}{\sqrt{2\pi}} e^{-\frac{(u-1)^2}{2}}
    \end{align*}
    And we can easily see that this joint density can be factorized into $g_1(u) = \frac{1}{\sqrt{2\pi}} e^{-\frac{(u-1)^2}{2}}, \quad g_2(v) = 1$. So, $Y/X$ and $X$ are independent.
    \end{enumerate}

    \section*{4.42}
    Given that $X$ and $Y$ are independent random variables, we could have,
    \begin{align*}
    \rho & = \frac{Cov(XY, Y)}{\sqrt{Var XY Var Y}} = \frac{EXY^2 - EXYEY}{\sqrt{(E(XY)^2 - (EXY)^2)Var Y}} \\
    & = \frac{EXEY^2 - EX(EY)^2}{\sqrt{(EX^2EY^2 - (EX)^2(EY)^2)Var Y}} \\
    & = \frac{\mu_X (\sigma_Y^2 + \mu_Y^2) - \mu_X \mu_Y^2}{\sqrt{\big((\sigma^2_X + \mu_X^2)(\sigma^2_Y + \mu_Y^2)-\mu_X^2\mu_Y^2\big)\sigma^2_Y}} \\
    & = \frac{\mu_X\sigma_Y}{\sqrt{\sigma^2_X\sigma^2_Y + \mu_X^2\sigma^2_Y + \mu_Y^2\sigma^2_X}}
    \end{align*}
    \section*{4.45}
    \begin{enumerate}[(a)]
    \item The pdf of a bivariate normal distribution given parameter $\mu_X, \mu_Y, \sigma_X^2, \sigma^2_Y, \rho$ is,
    \[
    f(x, y) = \frac{1}{2\pi\sigma_X\sigma_Y \sqrt{1-\rho^2}} \exp\left(-\frac{1}{2(1-\rho^2)} \left(\frac{(x-\mu_X)^2}{\sigma_X^2} - \frac{2\rho(x-\mu_X)(y-\mu_Y)}{\sigma_X \sigma_Y} + \frac{(y-\mu_Y)^2}{\sigma_Y^2}\right) \right)
    \]
    So, the marginal pdf $f_X(x)$ is,
    \begin{align*}
    f(x) & = \intii f(x,y) dy \\
    & = \frac{1}{\sqrt{2\pi}\sigma_X} \exp\left(\frac{1}{2(1-\rho^2)} (1-\rho^2)\frac{(x-\mu_X)^2}{\sigma_X^2}\right) \intii \frac{1}{\sqrt{2\pi}\sigma_Y \sqrt{1-\rho^2}} \exp \left(\frac{1}{1-\rho^2} \left( \frac{y-\mu_Y}{\sigma_Y} - \rho \frac{x-\mu_X}{\sigma_X} \right)^2 \right) dy \\
    & = \frac{1}{\sqrt{2\pi}\sigma_X} e^{-\frac{(x-\mu_X)^2}{2\sigma_X^2}} \intii \frac{1}{\sqrt{2\pi}\sigma_Y \sqrt{1-\rho^2}} e^{-\cfrac{\left(y-(\mu_Y +\rho \frac{\sigma_Y(x-\mu_X)}{\sigma_X}) \right)^2}{2(1-\rho^2)\sigma_Y^2}  } dy \\
    \end{align*}
    Notice that the integrand in the second term is a normal density, so it will integrate to 1. Thus, 
    \[
    f(x) = \frac{1}{\sqrt{2\pi}\sigma_X} e^{-\frac{(x-\mu_X)^2}{2\sigma_X^2}}
    \]
    \emph{i.e.} $X$ has marginal distribution of $N(\mu_X, \sigma_X^2)$.

    Since $X$ and $Y$ are equivalent and interchangable in $f(x,y)$, so the marginal distribution of $Y$ should be $N(\mu_Y, \sigma^2_Y)$.
    \item 
    \begin{align*}
    f(Y|X=x) & = \frac{f_{X,Y}(x,y)}{f_X(x)} \\
    & = \cfrac{\frac{1}{2\pi\sigma_X\sigma_Y \sqrt{1-\rho^2}} \exp\left(-\frac{1}{2(1-\rho^2)} \left(\frac{(x-\mu_X)^2}{\sigma_X^2} - \frac{2\rho(x-\mu_X)(y-\mu_Y)}{\sigma_X \sigma_Y} + \frac{(y-\mu_Y)^2}{\sigma_Y^2}\right) \right)}{\frac{1}{\sqrt{2\pi}\sigma_X}\exp\left(-\frac{(x-\mu_X)^2}{2\sigma_X^2}\right)} \\
    & = \frac{1}{\sqrt{2\pi}\sigma_Y\sqrt{1-\rho^2}} e^{-\cfrac{1}{2(1-\rho^2)} \left(\rho \cfrac{(x-\mu_X)^2}{\sigma_X^2} - \cfrac{2\rho(x - \mu_X)(y - \mu_Y)}{\sigma_X \sigma_Y} + \cfrac{(y-\mu_Y)^2}{\sigma_Y^2}\right)} \\
    & = \frac{1}{\sqrt{2\pi}\sigma_Y\sqrt{1-\rho^2}} e^{-\cfrac{1}{2(1-\rho^2)} \left(\rho \cfrac{\sigma_Y^2(x-\mu_X)^2}{\sigma_Y^2\sigma_X^2} - \cfrac{2\rho\sigma_Y(x - \mu_X)(y - \mu_Y)}{\sigma_X \sigma_Y^2} + \cfrac{(y-\mu_Y)^2}{\sigma_Y^2}\right)} \\
    & = \frac{1}{\sqrt{2\pi}\sigma_Y\sqrt{1-\rho^2}} e^{-\cfrac{\left((y-\mu_Y) - \frac{\rho\sigma_Y (x-\mu_X)}{\sigma_X}\right)^2}{2\sigma^2(1-\rho^2)}}
    \end{align*}
    And this is the pdf for $N(\mu_Y + \rho(x-\mu_X)\frac{\sigma_Y}{\sigma_X}, \sigma^2_Y(1-\rho^2))$.
    \end{enumerate}
    \section*{4.46}
    \begin{enumerate}[(a)]
    \item Because $Z_1$ and $Z_2$ are independent $N(0,1)$ random variables,and $a_X, b_X, c_X, a_Y, b_Y, c_Y$ are all constants, we can have,
    \begin{align*}
    E(Z_i) & = 0 \quad Var(Z_i) = 1 \\
    EX & = E(a_X Z_1 + b_X Z_2 + c_X) = a_X E(Z_1) + b_X E(Z_2) + c_X = c_X \\
    Var X & = Var(a_X Z_1 + b_X Z_2 + c_X) = a_X^2 E(Z_1) + b_X^2 E(Z_2) = a_X^2 + b_X^2 \\
    EY & = E(a_Y Z_1 + b_Y Z_2 + c_Y) = a_Y E(Z_1) + b_Y E(Z_2) + c_Y = c_Y \\
    Var Y & = Var(a_Y Z_1 + b_Y Z_2 + c_Y) = a_Y^2 E(Z_1) + b_Y^2 E(Z_2) = a_Y^2 + b_Y^2 \\
    Cov(X,Y) & = EXY - EXEY\\
    &= E\big(a_Xa_Y Z_1^2 + (a_Xb_Y + b_Xa_Y) Z_1Z_2 + b_X b_Y Z_2^2 + \\
    & + c_Xc_Y + c_Xa_YZ_2 + c_Xb_YZ_2 + c_Ya_XZ_1 + c_Yb_XZ_1\big) - c_Xc_Y \\
    \end{align*}
    Given that 
    \[
    E(Z_i^2) = \intii z^2 \frac{1}{\sqrt{2\pi}} e^{-z^2/2} dz = \left.\frac{1}{\sqrt{2\pi}} z e^{-z^2/2} \right|^{-\infty}_\infty + \intii \frac{1}{\sqrt{2\pi}} e^{-z^2/2} dz = 1,
    \]
    because the integrand is a normal pdf, and that
    \[
    E(Z_1Z_2) = E(Z_1)E(Z_2) = 0,
    \]
    we have,
    \[
    Cov(X, Y) = a_Xa_Y + b_X b_Y + c_Xc_Y - c_Xc_Y = a_Xa_Y + b_Xb_Y
    \]
    \item Simply plug in following constants into the expressions we derived in (a),
    \begin{align*}
    a_X = \sqrt{\frac{1+\rho}{2}} \sigma_X,  & \quad b_X = \sqrt{\frac{1-\rho}{2}} \sigma_X, & c_X = \mu_X \\
    a_Y = \sqrt{\frac{1+\rho}{2}} \sigma_Y,  & \quad b_Y = -\sqrt{\frac{1-\rho}{2}} \sigma_Y, & c_Y = \mu_Y \\
    \end{align*}
    we will get,
    \begin{align*}
    EX = c_X = \mu_X, \quad & Var X = a_X^2 + b_X^2 = \frac{1+\rho}{2} \sigma_X^2 + \frac{1-\rho}{2} \sigma_X^2 = \sigma_X^2, \\
    EY = c_Y = \mu_Y, \quad & Var Y = a_Y^2 + b_Y^2 = \frac{1+\rho}{2} \sigma_Y^2 + \frac{1-\rho}{2} \sigma_Y^2 = \sigma_Y^2, \\
    \end{align*}
    \[
    \rho_{XY} = \frac{Cov(X,Y)}{\sigma_X \sigma_Y} =\frac{a_X a_Y + b_X b_Y}{\sigma_X \sigma_Y} = \frac{\frac{1+\rho}{2} \sigma_X \sigma_Y - \frac{1-\rho}{2} \sigma_X \sigma_Y}{\sigma_X \sigma_Y} = \rho.
    \]

    \item 
    Provided that,
    \begin{align*}
    X & = a_X Z_1 + b_X Z_2 + c_X \\
    & = \sqrt{\frac{1+\rho}{2}} \sigma_X Z_1 + \sqrt{\frac{1-\rho}{2}} \sigma_X Z_1 + c_X \\
    Y & = a_Y Z_1 + b_Y Z_2 + c_Y \\
    & = \sqrt{\frac{1+\rho}{2}} \sigma_Y Z_1 - \sqrt{\frac{1-\rho}{2}} \sigma_Y Z_1 + c_Y \\
    \\
    a_Y X + a_X Y & = 2 a_X a_Y Z_1 + a_Y c_X + a_X c_Y + (a_X b_Y + a_Y b_X) Z_2 \\
    & = 2 a_X a_Y Z_1 + a_X c_Y + a_Y c_X \\
    \iff Z_1 & = \frac{a_Y (X-c_X) + a_X (Y - c_Y)}{2a_Xa_Y} \\
    & = \frac{\sqrt{\frac{1+\rho}{2}} (\sigma_Y(X-\mu_X) + \sigma_X(Y-\mu_Y))}{(1+\rho) \sigma_X \sigma_Y} \\
    & = \frac{\sigma_Y(X-\mu_X) + \sigma_X(Y-\mu_Y)}{\sqrt{2(1+\rho)}\sigma_X \sigma_Y} \\
    \end{align*}
    Plug in $Z_1$ into expression of $X$ and $Y$,
    \begin{align*}
    X & = a_X Z_1 + b_X Z_2 + c_X\\
    & = \sqrt{\frac{1+\rho}{2}} \sigma_X \frac{\sigma_Y(X-\mu_X) + \sigma_X(Y-\mu_Y)}{\sqrt{2(1+\rho)}\sigma_X \sigma_Y} + b_X Z_2 + \mu_X \\
    & = \frac{\sigma_Y(X-\mu_X) + \sigma_X (Y - \mu_Y)}{2 \sigma_Y} + b_X Z_2 + \mu_X\\
    \\
    Y & = a_Y Z_1 + b_Y Z_2 + c_Y\\
    & = \sqrt{\frac{1+\rho}{2}} \sigma_Y \frac{\sigma_Y(X-\mu_X) + \sigma_X(Y-\mu_Y)}{\sqrt{2(1+\rho)}\sigma_X \sigma_Y} + b_Y Z_2 + \mu_Y \\
    & = \frac{\sigma_Y(X-\mu_X) + \sigma_X (Y - \mu_Y)}{2 \sigma_X} + b_Y Z_2 + \mu_Y\\
    \\ 
    & \text{So,}\\
    (b_X + b_Y) Z_2 & = (X - \mu_X)/2 + (Y-\mu_Y)/2 - \frac{\sigma_X}{2\sigma_Y}(Y-\mu_Y) - \frac{\sigma_Y}{2\sigma_X}(X-\mu_X) \\
    \iff Z_2 & = \frac{(X-\mu_X) (\frac{\sigma_X - \sigma_Y}{\sigma_X}) + (Y-\mu_Y) (\frac{\sigma_Y-\sigma_X}{\sigma_Y})}{\sqrt{2(1-\rho)} (\sigma_X - \sigma_Y)} \\
    & = \frac{(X-\mu_X)/\sigma_X - (Y-\mu_Y)/\sigma_Y}{\sqrt{2(1-\rho)}} \\
    & = \frac{\sigma_Y(X-\mu_X) - \sigma_X(Y-\mu_Y)}{\sqrt{2(1-\rho)}\sigma_X \sigma_Y} \\
    \end{align*}

    The Jacobian is,
    \[
    J = \begin{vmatrix}
    \frac{\partial Z_1}{x} & \frac{\partial Z_1}{y}\\
    \frac{\partial Z_2}{x} & \frac{\partial Z_2}{y}\\
    \end{vmatrix} = -\frac{1}{\sqrt{1-\rho^2} \sigma_X \sigma_Y}
    \]

    Hence,
    \begin{align*}
    f(X, Y) & = f(Z_1)f(Z_2) |J|\\
    & = \frac{1}{2\pi} e^{-\frac{\left(\frac{\sigma_Y(X-\mu_X) + \sigma_X(Y-\mu_Y)}{\sqrt{2(1+\rho)}\sigma_X \sigma_Y}\right)^2}{2}} e^{-\frac{\left(\frac{\sigma_Y(X-\mu_X) - \sigma_X(Y-\mu_Y)}{\sqrt{2(1-\rho)}\sigma_X \sigma_Y}\right)^2}{2}} \frac{1}{\sqrt{2(1-\rho^2)}\sigma_X \sigma_Y} \\
    & = \frac{1}{2\pi\sqrt{1-\rho^2}\sigma_X\sigma_Y} \exp\Big\{-\big(\frac{(X-\mu_X)^2}{\sigma_X^2} + \frac{(Y-\mu_Y)^2}{\sigma_Y^2} \big) \big(\frac{1}{4(1+\rho)} + \frac{1}{4(1-\rho)} \big) \\
    & \quad + 2\frac{(X-\mu_X)(Y-\mu_Y)}{\sigma_X\sigma_Y}\left(\frac{1}{4(1+\rho)} - \frac{1}{4(1-\rho)}\right)\Big\} \\
    & = \frac{1}{2\pi\sqrt{1-\rho^2}\sigma_X\sigma_Y} \exp\left(-\frac{1}{2(1-\rho^2)}\left(\frac{(X-\mu_X)^2}{\sigma_X^2} + \frac{(Y-\mu_Y)^2}{\sigma_Y^2} -2\rho \frac{(X-\mu_X)(Y- \mu_Y)}{\sigma_X\sigma_Y} \right)\right), \\
    & \qquad -\infty < x, y < \infty
    \end{align*}
    As we can see, this is the bivariate normal density with parameters $\mu_X, \mu_Y, \sigma_X^2, \sigma_Y^2$ and $\rho$.

    \item Given equations,
    \begin{align*}
    \mu_X = c_X, \quad \sigma_X^2 = a_X^2 + b_X^2\\
    \mu_Y = c_Y, \quad \sigma_Y^2 = a_Y^2 + b_Y^2\\
    \rho \sigma_X \sigma_Y = a_X a_Y + b_Xb_Y
    \end{align*}
    Let $a_X = \pm \sqrt{\sigma_X^2 - b_X^2}, \quad a_Y = \pm \sqrt{\sigma_Y^2 - b_Y^2}$, we will have,
    \[
    \rho \sigma_X \sigma_Y = a_X a_Y + \pm \sqrt{\sigma_X^2 - b_X^2}\sqrt{\sigma_Y^2 - b_Y^2}
    \]
    which leads to,
    \[
    a_X^2 a_Y^2 + \rho^2 \sigma_X^2 \sigma_Y^2 -2 \rho \sigma_X \sigma_Y a_X a_Y = (\sigma_X^2 - a_X^2)(\sigma_Y^2 - a_Y^2)
    \]
    and further leads to,
    \[
    \sigma_Y^2 a_X^2 + \sigma_X^2 a_Y^2 - 2\rho a_X a_Y \sigma_X \sigma_Y + (\rho^2 -1)\sigma_X^2 \sigma_Y^2  = 0
    \]

    And this is a general ellipse formula for variable $a_X, a_Y$. So, there will be infinite solutions for $a_X$ and $a_Y$ and consequently infinite solutions too for $b_X, b_Y$.
    \end{enumerate}
\end{document}
